backend/Debugvarproof.v
@@ -606,6 +606,23 @@ Proof.
   eexact transf_final_states.
   eexact transf_step_correct.
 Qed.
+Lemma atx_sim:
+      simulation_atx
+        (fun (idx s1 : Smallstep.state (semantics prog))
+           (s2 : Smallstep.state (semantics tprog))
+         => idx = s1 /\ match_states s1 s2).
+Proof.
+  atx_sim_start_proof.
+  monadInv H0. 
+  eapply external_call_symbols_preserved in H8;
+    try apply senv_preserved.
+  repeat (econstructor; eauto).
+Qed.
+Lemma atx_preserved:
+  preserves_atx
+    (fun (idx s1 : Smallstep.state (semantics prog)) (s2 : Smallstep.state (semantics tprog))
+     => idx = s1 /\ match_states s1 s2).
+Proof. atx_preserved_start_proof. Qed.
 
 Theorem transf_program_correct:
   @fsim_properties_ext
@@ -613,9 +630,9 @@ Theorem transf_program_correct:
     get_mem get_mem.
 Proof.
   eapply EqEx_sim'; eapply sim_eqSim'; try eapply transf_program_correct'.
-  - admit.
-  - admit.
+  - exact atx_sim.
+  - exact atx_preserved.
   - simpl; intros ? ? ? [? ?]; subst; destruct H0; auto.
-Admitted.
+Qed.
 
 End PRESERVATION.
