common/Separation.v
@@ -899,7 +899,7 @@ Lemma external_call_parallel_rule_strong:
   /\ m2' |= minjection j' m1' ** globalenv_inject ge j' ** P
   /\ inject_incr j j'
   /\ inject_separated j j' m1 m2
-  /\ inject_trace j' t t' /\
+  /\ inject_trace_strong j' t t' /\
     injection_full j' m1' .
 Proof.
   intros until vargs2; intros CALL INJFULL SEP ARGS.
